pda/ogdensLemmaScript.sml
@@ -1,0 +1,374 @@
+open HolKernel boolLib bossLib Parse BasicProvers Defn
+
+open pred_setTheory stringTheory containerTheory relationTheory
+listTheory rich_listTheory optionTheory arithmeticTheory
+
+
+open listLemmasTheory relationLemmasTheory grammarDefTheory
+     arithmeticLemmasTheory symbolDefTheory cnfTheory parseTreeTheory
+     treeDerivTheory containerLemmasTheory pumpingLemmaTreeTheory
+
+val _ = new_theory "ogdensLemma";
+
+val _ = Globals.linewidth := 60
+val _ = set_trace "Unicode" 1
+
+fun MAGIC (asl, w) = ACCEPT_TAC (mk_thm(asl,w)) (asl,w);
+
+val marked = Define
+`marked P l = LENGTH (FILTER P l)`;
+
+val maxSp = Define
+`(maxSp P (Leaf ts) = []) ∧
+(maxSp P (Node nt [t1]) = []) ∧
+ (maxSp P (Node nt [t1;t2]) = 
+  if (marked P (leaves t1) ≤ marked P (leaves t2)) 
+      then 1::maxSp P t2
+  else 0::maxSp P t1)`;
+
+
+val countDistLeaves = Define
+`(countDistLeaves P (Leaf ts)  = []) ∧
+ (countDistLeaves P (Node nt stl) = MAP (marked P) (MAP leaves stl))`;
+
+val branchPoints = Define
+`(branchPoints P [] t = []) ∧
+(branchPoints P (p::path) (Node nt [Node n1 t1; Node n2 t2]) = 
+ if (LENGTH (FILTER (λn. n = 0) 
+	     (countDistLeaves P (Node nt [Node n1 t1; Node n2 t2]))) = 0)
+     then (Node nt [Node n1 t1; Node n2 t2])::
+	 branchPoints P path (EL p [Node n1 t1; Node n2 t2])
+ else branchPoints P path (EL p [Node n1 t1; Node n2 t2])) ∧
+ (branchPoints P path t = [])`;
+
+
+val markedApp = store_thm
+("markedApp",
+``∀l1 l2. marked P (l1 ++ l2) = marked P l1 + marked P l2``,
+
+Induct_on `l1` THEN SRW_TAC [][marked] THEN
+FULL_SIMP_TAC (srw_ss()) [marked, FILTER_APPEND] THEN
+DECIDE_TAC);
+
+
+val bpImpMarked = store_thm
+("bpImpMarked",
+``∀g t. validptree g t ⇒ isCnf g ⇒ 
+∀k. LENGTH (branchPoints P (maxSp P t) t) ≤ k ⇒
+marked P (leaves t) ≤ 2**k``,
+
+HO_MATCH_MP_TAC validptree_ind THEN SRW_TAC [][] 
+THENL[
+      IMP_RES_TAC cnfTree THEN
+      FULL_SIMP_TAC (srw_ss()) [] THEN SRW_TAC [][] THENL[
+
+      FULL_SIMP_TAC (srw_ss()) [maxSp] THEN
+      Cases_on `marked P (leaves (Node n1 t1)) ≤ marked P (leaves (Node n2 t2))` THEN
+      FULL_SIMP_TAC (srw_ss()) [] THEN1
+      (`validptree g (Node n2 t2)` by 
+       FULL_SIMP_TAC (srw_ss()) [validptree, isNode_def] THEN
+      FIRST_X_ASSUM (Q.SPECL_THEN [`Node n2 t2`] MP_TAC) THEN 
+       SRW_TAC [][isNode_def] THEN
+      FIRST_X_ASSUM (Q.SPECL_THEN [`k`] MP_TAC) THEN SRW_TAC [][] THEN
+      FULL_SIMP_TAC (srw_ss()) [branchPoints] THEN
+      Cases_on `LENGTH
+      (FILTER (λn. n = 0)
+       (countDistLeaves P
+	(Node n [Node n1 t1; Node n2 t2]))) = 0` THEN
+      FULL_SIMP_TAC (srw_ss()) [] THEN
+      `LENGTH
+      (branchPoints P (maxSp P (Node n2 t2))
+       (Node n2 t2)) ≤ k` by DECIDE_TAC THEN
+      FULL_SIMP_TAC (srw_ss()) [leaves_def] THEN
+      FULL_SIMP_TAC (srw_ss()) [markedApp] THEN DECIDE_TAC
+      MAGIC) THEN
+
+      (`validptree g (Node n1 t1)` by 
+       FULL_SIMP_TAC (srw_ss()) [validptree, isNode_def] THEN
+      FIRST_X_ASSUM (Q.SPECL_THEN [`Node n1 t1`] MP_TAC) THEN 
+       SRW_TAC [][isNode_def] THEN
+      FIRST_X_ASSUM (Q.SPECL_THEN [`k`] MP_TAC) THEN SRW_TAC [][] THEN
+      FULL_SIMP_TAC (srw_ss()) [branchPoints] THEN
+      Cases_on `LENGTH
+      (FILTER (λn. n = 0)
+       (countDistLeaves P
+	(Node n [Node n1 t1; Node n2 t2]))) = 0` THEN
+      FULL_SIMP_TAC (srw_ss()) [] THEN
+      `LENGTH
+      (branchPoints P (maxSp P (Node n1 t1))
+       (Node n1 t1)) ≤ k` by DECIDE_TAC THEN
+      FULL_SIMP_TAC (srw_ss()) [leaves_def] THEN
+      MAGIC),
+
+      FULL_SIMP_TAC (srw_ss()) [validptree, branchPoints, maxSp,
+				leaves_def, marked] THEN
+      SRW_TAC [][] THEN
+      MAGIC],
+
+      FULL_SIMP_TAC (srw_ss()) [validptree]
+      ]);
+
+
+val validCnfPath = Define `validCnfPath p = ∀e. e ∈ p ⇒ (e=0) ∨ (e=1)`;
+
+(*
+``∀g t. validptree g t ⇒ isCnf g ⇒
+∀bps p. (bps = (branchPoints P p t)) ⇒ 
+validCnfPath p ⇒
+∀i. i < LENGTH bps ⇒ 
+(∀j. j > i ∧ j < LENGTH bps ⇒ isSubtree (EL j bps) (EL i bps))``,
+
+HO_MATCH_MP_TAC validptree_ind THEN SRW_TAC [][] THENL[
+
+IMP_RES_TAC cnfTree THEN
+FULL_SIMP_TAC (srw_ss()) [] THEN SRW_TAC [][] THEN
+Cases_on `p` THEN FULL_SIMP_TAC (srw_ss()) [branchPoints] THEN
+SRW_TAC [][] THEN FULL_SIMP_TAC (srw_ss()) [] THEN1
+
+Cases_on `i` THEN FULL_SIMP_TAC (srw_ss()) [] THEN
+FULL_SIMP_TAC (srw_ss()) [validCnfPath] THEN
+`(h = 0) ∨ (h=1)` by METIS_TAC [] THEN FULL_SIMP_TAC (srw_ss()) [] THEN
+SRW_TAC [][] THEN1
+
+`validptree g (Node n1 t1)` by FULL_SIMP_TAC (srw_ss()) [validptree, isNode_def] THEN
+FIRST_X_ASSUM (Q.SPECL_THEN [`Node n1 t1`] MP_TAC) THEN SRW_TAC [][isNode_def] THEN
+FIRST_X_ASSUM (Q.SPECL_THEN [`t`] MP_TAC) THEN SRW_TAC [][] THEN
+Cases_on `j` THEN FULL_SIMP_TAC (srw_ss()) [] THEN
+FIRST_X_ASSUM (Q.SPECL_THEN [`n'`] MP_TAC) THEN SRW_TAC [][] THEN
+SRW_TAC [][isSubtree_def]
+
+
+Cases_on `j` THEN FULL_SIMP_TAC (srw_ss()) [] THEN
+
+*)
+
+
+val memBpsSubEq = store_thm
+("memBpsSubEq",
+``∀g t. validptree g t ⇒ isCnf g ⇒
+∀p. validCnfPath p ⇒
+∀bps. (bps = (branchPoints P p t)) ⇒ 
+∀e. e ∈ bps ⇒ isSubtreeEq e t``,
+
+HO_MATCH_MP_TAC validptree_ind THEN SRW_TAC [][]
+THENL[
+      IMP_RES_TAC cnfTree THEN
+      FULL_SIMP_TAC (srw_ss()) [] THEN SRW_TAC [][] THEN
+      Cases_on `p` THEN FULL_SIMP_TAC (srw_ss()) [branchPoints] THEN
+      SRW_TAC [][] THEN FULL_SIMP_TAC (srw_ss()) [] THEN
+      Cases_on `LENGTH
+          (FILTER (λn. n = 0)
+             (countDistLeaves P
+                (Node n [Node n1 t1; Node n2 t2]))) =
+        0` THEN FULL_SIMP_TAC (srw_ss()) [] THEN
+      SRW_TAC [][] THEN1
+      METIS_TAC [isSubEqImpSub] THEN
+      (FULL_SIMP_TAC (srw_ss()) [validCnfPath] THEN
+      `(h = 0) ∨ (h=1)` by METIS_TAC [] THEN FULL_SIMP_TAC (srw_ss()) [] THEN
+      SRW_TAC [][] 
+      THENL[
+	    `validptree g (Node n1 t1)` 
+	    by FULL_SIMP_TAC (srw_ss()) [validptree, isNode_def] THEN
+	    FIRST_X_ASSUM (Q.SPECL_THEN [`Node n1 t1`] MP_TAC) THEN
+	    SRW_TAC [][isNode_def] THEN
+	    `isSubtreeEq e (Node n1 t1)` by METIS_TAC [] THEN
+	    `isSubtree (Node n1 t1) (Node n [Node n1 t1; Node n2 t2])` by
+	    (SRW_TAC [][isSubtree_def] THEN
+	     Q.EXISTS_TAC `[0]` THEN SRW_TAC [][subtree_def]) THEN
+	    METIS_TAC [isSubEqImpSub, subtreeTrans],
+
+	    `validptree g (Node n2 t2)` 
+	    by FULL_SIMP_TAC (srw_ss()) [validptree, isNode_def] THEN
+	    FIRST_X_ASSUM (Q.SPECL_THEN [`Node n2 t2`] MP_TAC) THEN
+	    SRW_TAC [][isNode_def] THEN
+	    `isSubtreeEq e (Node n2 t2)` by METIS_TAC [] THEN
+	    `isSubtree (Node n2 t2) (Node n [Node n1 t1; Node n2 t2])` by
+	    (SRW_TAC [][isSubtree_def] THEN
+	     Q.EXISTS_TAC `[1]` THEN SRW_TAC [][subtree_def]) THEN
+	    METIS_TAC [isSubEqImpSub, subtreeTrans]
+	    ]),
+
+      FULL_SIMP_TAC (srw_ss()) [validptree]
+      ]);
+
+
+val bpsApp = store_thm
+("bpsApp",
+``∀bps p t. (bps = (branchPoints P p t)) ⇒ bps ≠ [] ⇒
+validCnfPath p ⇒
+∃pfx sfx st. (p = pfx ++ sfx) ∧ (subtree t pfx = SOME st) ∧
+(bps = branchPoints P pfx t ++ branchPoints P sfx st)``,
+
+Induct_on `p` THEN SRW_TAC [][] THEN1
+FULL_SIMP_TAC (srw_ss()) [branchPoints] THEN
+`∃n n1 t1 n2 t2. (t = Node n [Node n1 t1; Node n2 t2])` by MAGIC THEN
+SRW_TAC [][] THEN
+FULL_SIMP_TAC (srw_ss()) [branchPoints] THEN
+SRW_TAC [][] THEN FULL_SIMP_TAC (srw_ss()) [] THEN1
+
+(Q.EXISTS_TAC `[]` THEN
+Q.EXISTS_TAC `h::p` THEN
+FULL_SIMP_TAC (srw_ss()) [branchPoints]) THEN
+
+`validCnfPath p` by METIS_TAC [validCnfPath, MEM] THEN
+FIRST_X_ASSUM (Q.SPECL_THEN [`EL h [Node n1 t1; Node n2 t2]`] MP_TAC) THEN
+SRW_TAC [][] THEN
+FULL_SIMP_TAC (srw_ss()) [validCnfPath] THEN
+`h < 2` by (`(h = 0) ∨ (h = 1)` by METIS_TAC [] THEN
+	    DECIDE_TAC) THEN
+Q.EXISTS_TAC `h::pfx` THEN
+Q.EXISTS_TAC `sfx` THEN
+Q.EXISTS_TAC `st` THEN
+FULL_SIMP_TAC (srw_ss()) [subtree_def] THEN
+FULL_SIMP_TAC (srw_ss()) [branchPoints]);
+
+
+val bpsApp = store_thm
+("bpsApp",
+``∀bps p t. (bps = (branchPoints P p t)) ⇒ bps ≠ [] ⇒
+validCnfPath p ⇒
+ ((∃i st. (subtree t [i] = SOME st) ∧ (bps = t :: branchPoints P (TL p) st)) ∨
+  (∃pfx sfx st. (pfx ≠ []) ∧ (p = pfx ++ sfx) ∧ (subtree t pfx = SOME st) ∧
+   (bps = st :: branchPoints P  sfx st)))``,
+
+completeInduct_on `ptheight t` THEN
+SRW_TAC [][] THEN
+`∃n n1 t1 n2 t2. (t = Node n [Node n1 t1; Node n2 t2])` by MAGIC THEN
+SRW_TAC [][] THEN
+FULL_SIMP_TAC (srw_ss()) [branchPoints] THEN
+SRW_TAC [][] THEN FULL_SIMP_TAC (srw_ss()) [] THEN
+`validCnfPath p` by METIS_TAC [validCnfPath, MEM] THEN
+Cases_on `p` THEN FULL_SIMP_TAC (srw_ss()) [branchPoints] THEN
+SRW_TAC [][] THEN FULL_SIMP_TAC (srw_ss()) [] THEN1
+`(h = 0) ∨ (h = 1)` by METIS_TAC [validCnfPath, MEM] THEN
+SRW_TAC [][] THEN
+FULL_SIMP_TAC (srw_ss()) [] THEN
+
+FIRST_X_ASSUM (Q.SPECL_THEN [`ptheight (Node n1 t1)`] MP_TAC) THEN SRW_TAC [][] THEN
+FULL_SIMP_TAC (arith_ss) [] THEN
+FIRST_X_ASSUM (Q.SPECL_THEN [`Node n1 t1`] MP_TAC) THEN SRW_TAC [][] THEN
+FULL_SIMP_TAC (arith_ss) [] THEN
+Cases_on `branchPoints P (0::t) (Node n1 t1) = []` THEN
+SRW_TAC [][] THEN1
+
+
+
+
+
+SRW_TAC [][] THEN1
+
+DISJ1_TAC THEN
+Q.EXISTS_TAC `[h]` THEN
+Q.EXISTS_TAC `p` THEN
+SRW_TAC [][]
+
+
+
+
+
+
+(Q.EXISTS_TAC `[]` THEN
+Q.EXISTS_TAC `h::p` THEN
+SRW_TAC [][branchPoints] THEN
+Q.EXISTS_TAC `h` THEN
+Q.EXISTS_TAC `EL h [Node n1 t1; Node n2 t2]` THEN
+SRW_TAC [][subtree_def] THEN
+`h < 2` by (`(h = 0) ∨ (h = 1)` by METIS_TAC [validCnfPath, MEM] THEN
+	    DECIDE_TAC)) THEN
+
+
+
+
+
+
+
+
+
+``∀bps p t. (bps = (branchPoints P p t)) ⇒ 
+¬ (ALL_DISTINCT (MAP root bps)) ⇒
+∃pfx m sfx t1 t2. (bps = pfx ++ [t1] ++ m ++ [t2] ++ sfx) ∧
+rootRep t2 t1 ∧ (∀st. ¬rootRep st t2)``,
+
+Induct_on `bps` THEN SRW_TAC [][] THEN
+
+Cases_on `t` THEN Cases_on `p` THEN
+FULL_SIMP_TAC (srw_ss()) [branchPoints] THEN
+Cases_on `LENGTH
+          (FILTER (λn. n = 0)
+             (countDistLeaves P (Node n l))) =
+        0` THEN FULL_SIMP_TAC (srw_ss()) [] THEN
+SRW_TAC [][] THENL[
+
+
+
+
+FIRST_X_ASSUM (Q.SPECL_THEN [`t`,`EL h' l`] MP_TAC) THEN SRW_TAC [][] THEN
+Cases_on `¬ALL_DISTINCT
+         (MAP root (branchPoints P t (EL h' l)))` THEN1
+METIS_TAC [APPEND] THEN
+FULL_SIMP_TAC (srw_ss()) [] THEN
+FULL_SIMP_TAC (srw_ss()) [MEM_MAP] THEN
+IMP_RES_TAC rgr_r9eq THEN
+SRW_TAC [][rootRep_def] THEN
+`isSubtreeEq y (EL h' l)` by METIS_TAC [memBpsSubEq] THEN
+`isSubtree (EL h' l) (Node n l)`by MAGIC THEN
+MAGIC
+
+
+
+``∀bps. bps ≠ [] ⇒
+(bps = branchPoints P (maxSp P t) t) ⇒ ALL_DISTINCT (MAP root bps) ⇒
+      (∃ntl ntl1 ntl2. (LAST bps = Node ntl [ntl1;ntl2]) ∧
+      ∃ntm pfx sfx. (bps = pfx ++ [ntm] ++ sfx) ∧ rootRep ntl1 ntm ∧
+      ∀e. e ∈ sfx ⇒ root e ≠ root ntm)``
+
+Induct_on `bps` THEN SRW_TAC [][] THEN
+Cases_on `bps` THEN FULL_SIMP_TAC (srw_ss()) [] THEN
+SRW_TAC [][] THEN
+
+
+
+
+
+
+
+val ogdensLemma = store_thm
+("ogdensLemma",
+``∀g.
+   isCnf (g:('a,'b) grammar)  ⇒
+   ∃n. n > 0 ∧
+       ∀z. z ∈ language g ∧ marked P (MAP tsToStr z) ≥ n ⇒
+           ∃u v w x y.
+             (z = u ++ v ++ w ++ x ++ y) ∧
+             marked P (MAP ts2str (v++x)) ≥ 1 ∧
+	     marked P (MAP ts2str (v++w++x)) ≤ n ∧
+             ∀i. u ++ FLAT (lpow v i) ++ w ++ FLAT (lpow x i) ++ y ∈ language g``,
+
+SRW_TAC [][] THEN
+ Q.ABBREV_TAC `k=LENGTH (ntms g)` THEN
+ Q.EXISTS_TAC `2**k + 1` THEN
+SRW_TAC [][] THEN1
+MAGIC THEN
+
+`∃t. validptree g t ∧ (root t = NTS (startSym g)) ∧ (z = MAP TS (leaves t))` 
+ by METIS_TAC [ptLangThm, fringeEqLeaves] THEN
+SRW_TAC [][] THEN
+Q.ABBREV_TAC `p = maxSp P t` THEN
+Q.ABBREV_TAC `bps = branchPoints P (maxSp P t) t` THEN
+`LENGTH bps ≥ k` by MAGIC THEN
+Cases_on `ALL_DISTINCT (MAP root bps)`
+THENL[
+      `∃ntl ntl1 ntl2. (LAST bps = Node ntl [ntl1;ntl2]) ∧
+      ∃ntm pfx sfx. (bps = pfx ++ [ntm] ++ sfx) ∧ rootRep ntl1 ntm ∧
+      ∀e. e ∈ sfx ⇒ root e ≠ root ntm` by MAGIC THEN
+      SRW_TAC [][] THEN
+      
+      
+
+
+
+
+      ]
+
+
+val _ = export_theory ();
