slr-parsing/followSetDefScript.sml
@@ -20,6 +20,57 @@ val followSet = Define
 { TS ts | ∃s.MEM s (MAP ruleRhs (rules g)) ∧ 
           ∃pfx sfx.RTC (derives g) s (pfx++[sym]++[TS ts]++sfx) }`;
 
+
+val followML_defn = Hol_defn "followML"
+  `(followG g sn N = followrs g sn N (rules g)) ∧
+   (followrs g sn N [] = {}) ∧
+   (followrs g sn N (r::rs) =
+      followr g sn N (ruleLhs r) (ruleRhs r) ∪
+      followrs g sn N rs) ∧
+   (followr g sn N M [] = {}) ∧
+   (followr g sn N M (TS t::rest) = followr g sn N M rest) ∧
+   (followr g sn N M (NTS P :: rest) =
+      (if N = P then
+         firstSetList g rest ∪
+         (if nullableML g [] rest then
+            if M ∈ sn ∨ NTS M ∉ nonTerminals g ∨
+               ¬(IMAGE NTS (set sn) ⊆ nonTerminals g) then {}
+            else followG g (N::sn) M
+          else {})
+       else {}) ∪ followr g sn N M rest)`
+
+val easy_def = Define`
+  (easy (INL _) = 0) ∧
+  (easy (INR (INL (_, _, _, rs))) = LENGTH rs) ∧
+  (easy (INR (INR (_, _, _, _, syms))) = LENGTH syms)
+`
+
+val cg_def = Define`
+  (cg (INL _) = 2) ∧
+  (cg (INR (INL _)) = 1) ∧
+  (cg (INR (INR _)) = 0)
+`;
+
+val tricky_def = Define`
+  tricky (g,sn) = CARD (nonTerminals g) - LENGTH sn
+`;
+
+val gsn_def = Define`
+  (gsn (INL (g,sn,_)) = (g,sn)) ∧
+  (gsn (INR (INL (g,sn,_))) = (g,sn)) ∧
+  (gsn (INR (INR (g,sn,_))) = (g,sn))`
+
+val (followML_def, followML_ind) = tprove(
+  followML_defn,
+  WF_REL_TAC `inv_image (measure tricky LEX $< LEX measure easy)
+                        (λx. (gsn x, cg x, x))` THEN
+  SRW_TAC [][gsn_def, cg_def, easy_def, tricky_def] THEN1 DECIDE_TAC THEN
+  ...
+
+
+
+
+
 val followRuleML_defn = Hol_defn "followRuleML_defn"
 `(followRuleML g sn sym (rule l []) = {}) ∧
 (followRuleML g sn sym (rule l (h::t)) = 
@@ -280,7 +331,7 @@ val lemma' =  SIMP_RULE (srw_ss() ++ boolSimps.DNF_ss) []
 		       ntderive'_list_exists 
 
 
-
+(*
 ``s ∈ followSet g sym ⇒ s ∈ followSetML g sym``,
 
 SRW_TAC [][followSet] THEN
@@ -332,6 +383,7 @@ IMP_RES_TAC
 
 
 ``∀g sn sf. ts ∈ firstSet1 g sn sf ⇒ ts ∈ followSet ``
+*)
 
 val mlDir = ref ("./theoryML/");
 
