slr-parsing/macStepScript.sml
@@ -4,7 +4,7 @@ open listTheory containerTheory pred_setTheory arithmeticTheory
 relationTheory markerTheory boolSimps optionTheory rich_listTheory
 pairTheory
 
-open regexpTheory grammarDefTheory boolLemmasTheory listLemmasTheory
+open symbolDefTheory grammarDefTheory boolLemmasTheory listLemmasTheory
 setLemmasTheory whileLemmasTheory parseTreeTheory followSetDefTheory
 yaccDefTheory parseProp1DefTheory parseProp2DefTheory
 lrGrammarDefTheory validItemInvTheory
