slr-parsing/parseProp2DefScript.sml
@@ -3,7 +3,7 @@ open HolKernel boolLib bossLib Parse BasicProvers Defn
 open listTheory containerTheory pred_setTheory arithmeticTheory
 relationTheory markerTheory boolSimps optionTheory
 
-open regexpTheory grammarDefTheory boolLemmasTheory listLemmasTheory
+open symbolDefTheory grammarDefTheory boolLemmasTheory listLemmasTheory
 parseTreeTheory yaccDefTheory parseProp1DefTheory
 
 
